Tealeaves/Examples/LambdaNominal/EquivalenceV1.v
@@ -554,3 +554,350 @@ Section rw.
 End rw.
 *)
 
+
+
+
+
+
+(*
+Lemma lemma2: forall
+    (conflicts: list name) (fv_u: list name) (x:name) (u: term name name),
+    (subst_from_context x u conflicts) ⦿ [x] =
+      ret ∘ extract.
+Proof.
+  intros.
+  ext (ctx, v).
+  unfold preincr, incr, compose.
+  change ([x] ● ctx) with (x::ctx).
+  unfold subst_from_context.
+  destruct (get_binding_spec (x :: ctx) v) as [[Heq Hnin]| H2].
+  - rewrite Heq.
+    assert (v <> x).
+    rewrite element_of_list_cons in Hnin. tauto.
+    destruct_eq_args v x.
+  - destruct H2 as [pre [post [rest1 [rest2 rest3]]]].
+    rewrite rest1.
+    cbn.
+    destruct pre.
+    + cbn. fequal.
+      assert (x = v).
+      { now inversion rest2. }
+      subst.
+      unfold rename_binder_one.
+      destruct_eq_args v v.
+    +
+      assert (x = n).
+      { now inversion rest2. }
+      subst.
+      change_left (ret ((rename_binder_from_context n conflicts ⦿ [n]) (pre, v))).
+      rewrite lemma1.
+      reflexivity.
+Qed.
+
+
+Section interpret.
+
+  Context
+    (conflicts: list name)
+    (fv_u: list name) (x: name) (u: term name name).
+
+  (*
+  Definition interpret_context_to_renamings  (context: list name):
+    term name name -> term name name :=
+    match context with
+    | nil => id
+    | cons b rest =>
+        if b == x
+        then id
+        else if SmartAtom.name_inb x
+             then let z := (fresh ([x] ++ l ++ [b]): name) in
+                  interpret_context_to_renamings rest ∘ rename b z
+             else id.
+
+    Definition interpret_context (conflicts: list name) (fv_u: list name) (x: name) (u: term name name) (context: list name):
+      term name name -> term name name :=
+      match context with
+      | nil => substF conflicts x u
+      | cons b rest =>
+          if b == x
+          then substF conflicts x u
+          else if SmartAtom.name_inb x
+               then substF (conflicts ++ context_to_renamed context) x u
+               else substF conflicts x u
+      end.
+
+Lemma equiv_key:
+  forall (conflicts: list name) (x: name) (u: term name name) (context: list name) (t: term name name),
+     substitute (T := term) (G := fun A => A)
+       (rename_binder_from_context x conflicts (FV term u) ⦿ context)
+       (subst_from_context x u conflicts (FV term u) ⦿ context) t =
+       interpret_context conflicts (FV term u) x u context t.
+Proof.
+  intros.
+  induction t.
+  - rewrite sub_term_rw1.
+    unfold preincr, incr, compose.
+    change (@nil name) with (Ƶ:list name).
+    rewrite monoid_id_l.
+    induction context.
+
+   *)
+
+Theorem woah:
+  forall (conflicts: list name) (x: name) (u: term name name) (b: name) (t: term name name),
+    (~ b ∈ fvL u ->
+     b <> x ->
+     substitute (T := term) (G := fun A => A)
+       (rename_binder_from_context x conflicts (FV term u) ⦿ [b])
+       (subst_from_context x u conflicts (FV term u) ⦿ [b]) t =
+       substF (conflicts ++ [b]) x u t) /\
+      (b ∈ fvL u ->
+       b <> x ->
+       substitute (T := term) (G := fun A => A)
+         (rename_binder_from_context x conflicts (FV term u) ⦿ [b])
+         (subst_from_context x u conflicts (FV term u) ⦿ [b]) t =
+         substF (conflicts ++ [fresh ([x] ++ conflicts ++ [b])]) x u
+           (rename (conflicts ++ [fresh ([x] ++ conflicts ++ [b])])  b (fresh ([x] ++ conflicts ++ [b])) t)).
+Proof.
+  intros.
+  generalize dependent conflicts.
+  generalize dependent b.
+  induction t.
+  - admit.
+  - (* λ b t *)
+Abort.
+
+
+Theorem subst_preincr_inFV_spec:
+  forall (conflicts: list name) (x: name) (u: term name name) (b: name) (t: term name name),
+      b ∈ fvL u ->
+      b <> x ->
+      substitute (T := term) (G := fun A => A)
+        (rename_binder_from_context x conflicts (FV term u) ⦿ [b])
+        (subst_from_context x u conflicts (FV term u) ⦿ [b]) t =
+        substF (conflicts ++ [fresh ([x] ++ conflicts ++ [b])]) x u
+          (rename (conflicts ++ [fresh ([x] ++ conflicts ++ [b])]) b (fresh ([x] ++ conflicts ++ [b])) t).
+Proof.
+  introv Hin Hneq.
+  generalize dependent conflicts.
+  generalize dependent b.
+  induction t; intros.
+  - rewrite sub_term_rw1.
+    rewrite rename_rw1.
+    destruct_eq_args v b.
+    + rewrite substF_rw1.
+      unfold preincr, incr, compose.
+      change ([b] ● []) with ([b]).
+      unfold subst_from_context.
+      assert (get_binding [b] b = Bound [] b []).
+      { cbn. destruct_eq_args b b. }
+      rewrite H.
+      assert (fresh ([x] ++ conflicts ++ [b]) <> x).
+      { intro contra.
+        assert (~ x ∈ ([x] ++ conflicts ++ [b])).
+        symmetry in contra.
+        rewrite contra at 1.
+        apply SmartAtom.fresh_not_in.
+        rewrite element_of_list_app in H0.
+        rewrite element_of_list_one in H0.
+        tauto.
+      }
+      destruct_eq_args (fresh ([x] ++ conflicts ++ [b])) x.
+      { intuition. }
+      { fequal.
+        unfold rename_binder_from_context.
+        unfold rename_binder_from_context_rec.
+        unfold rename_binder_one.
+        destruct_eq_args b x.
+        rewrite FV_fvL.
+        step_set_test.
+        rewrite List.app_nil_l.
+        admit.
+        admit.
+      }
+    +
+      unfold preincr, incr, compose.
+      change ([b] ● []) with ([b]).
+      unfold subst_from_context.
+      assert (get_binding [b] v = Unbound [b]).
+      { cbn. destruct_eq_args b v. }
+      rewrite H.
+      destruct_eq_args v x.
+      { rewrite substF_rw1.
+        destruct_eq_args x x.
+      }
+      { rewrite substF_rw1.
+        destruct_eq_args v x.
+      }
+  - rewrite sub_term_rw2.
+    simplify_applicative_I.
+    unfold ap, mult, Mult_I; unfold_ops @Map_I.
+    rewrite rename_rw2_neq.
+
+    rewrite substF_rw2.
+    admit.
+    admit.
+    admit.
+  - rewrite rename_rw3.
+    rewrite substF_rw3.
+    rewrite <- IHt1; auto.
+    rewrite <- IHt2; auto.
+Admitted.
+
+Lemma tvar_helper:
+  forall (conflicts: list name) (x: name) (u: term name name) (b: name) (t: term name name) v,
+    ~ b ∈ fvL u ->
+     b <> x ->
+     subst_from_context x u conflicts (FV term u) ([b], v) = (if v == x then u else tvar v).
+Proof.
+  intros.
+  cbn.
+  destruct_eq_args v b.
+  destruct_eq_args b x.
+  cbn.
+  unfold rename_binder_one.
+  destruct_eq_args b x.
+  rewrite FV_fvL.
+  step_set_test.
+  destruct (destruct_in b []).
+  inversion H2.
+  now step_set_test.
+Qed.
+
+
+Theorem subst_preincr_ninFV_spec:
+  forall (conflicts: list name) (x: name) (u: term name name) (b: name) (t: term name name),
+      ~ b ∈ fvL u ->
+      b <> x ->
+    substitute (T := term) (G := fun A => A)
+      (rename_binder_from_context x conflicts (FV term u) ⦿ [b])
+      (subst_from_context x u conflicts (FV term u) ⦿ [b]) t =
+      substF (conflicts ++ [b]) x u t.
+Proof.
+  introv Hnin Nneq.
+  generalize dependent conflicts.
+  generalize dependent b.
+  induction t; intros.
+  - rewrite sub_term_rw1.
+    rewrite substF_rw1.
+    unfold preincr, incr, compose.
+    change ([b] ● []) with ([b]).
+    rewrite tvar_helper; auto.
+  - rewrite sub_term_rw2.
+    simplify_applicative_I.
+    unfold ap, mult, Mult_I; unfold_ops @Map_I.
+    rewrite substF_rw2.
+
+    destruct_eq_args b x.
+    { fequal.
+      { unfold rename_binder_from_context.
+        unfold preincr, incr, compose.
+        change ([b0] ● []) with ([b0]).
+        cbn.
+        destruct_eq_args b0 x.
+        admit.
+      }
+      {
+        specialize (IHt b0 Hnin Nneq).
+        admit.
+      }
+    }
+    { destruct (SmartAtom.name_inb b (fvL u)).
+      admit.
+      admit.
+    }
+  - cbn.
+    rewrite substF_rw3.
+    rewrite <- IHt1.
+    rewrite <- IHt2.
+    reflexivity.
+Admitted.
+
+Theorem equivalence:
+  forall (conflicts: list name) (x: name) (u: term name name),
+    subst_top x u conflicts (FV term u) =
+      substF conflicts x u.
+Proof.
+  intros. ext t.
+  induction t.
+  - rewrite subst_top_rw1.
+    rewrite substF_rw1.
+    reflexivity.
+  - rewrite subst_top_rw2.
+    rewrite substF_rw2.
+    destruct_eq_args b x.
+    {
+      fequal.
+      { cbn.
+        unfold rename_binder_one.
+        destruct_eq_args x x.
+      }
+      {
+        rewrite lemma1.
+        unfold rename_binder_one.
+        rewrite lemma2.
+        rewrite kdtmp_substitute1.
+        reflexivity.
+      }
+    }
+    { destruct (destruct_in b (fvL u)).
+      { step_set_test.
+        fequal.
+        { unfold rename_binder_from_context.
+          rewrite rename_binder_from_context_rec_rw_nil.
+          unfold rename_binder_one.
+          destruct_eq_args b x.
+          rewrite FV_fvL.
+          step_set_test.
+          rewrite List.app_nil_l.
+          reflexivity.
+        }
+        {
+          apply subst_preincr_inFV_spec; auto.
+        }
+      }
+      { step_set_test.
+        fequal.
+        { cbn.
+          unfold rename_binder_one.
+          destruct_eq_args b x.
+          rewrite FV_fvL.
+          step_set_test.
+          destruct (destruct_in b []).
+          inversion H2.
+          now step_set_test.
+        }
+        {
+          rewrite subst_preincr_ninFV_spec; auto.
+        }
+      }
+    }
+  - cbn.
+    rewrite substF_rw3.
+    rewrite <- IHt1.
+    rewrite <- IHt2.
+    reflexivity.
+Qed.
+
+
+Lemma rename_binder_local_history_preincr_spec:
+  forall (conflicts: list name) (x:name) (fv_u: list name) (b:name),
+    b <> x ->
+    ~ (b ∈) ->
+  (rename_binder_local_history conflicts x ⦿ [b]) =
+    (rename_binder_local_history (conflicts ++ [b]) x).
+Proof.
+  introv BneqX BnotinFVu.
+  ext (ctx, v).
+  unfold preincr, compose, incr.
+  change (?a ● ?g) with (a ++ g).
+  unfold rename_binder_local_history.
+  destruct_eq_args x v.
+  destruct (SmartAtom.name_inb v).
+  - repeat rewrite List.app_assoc.
+    reflexivity.
+  - repeat rewrite List.app_assoc.
+    reflexivity.
+Qed.
+
+*)
